Progress on ghost task queue, instantiated the monotonic higher ghost reference interface, and started doing the reasoning with permissions

share/steel/examples/pulse/parallel/GhostTaskQueue.fst
@@ -1,23 +1,7 @@
 module GhostTaskQueue
 
-open FStar.List.Tot.Base
+module L = FStar.List.Tot.Base
 module P = FStar.Preorder
-
-// Mostly: Monotonic list of tasks with status
-
-type task_status = | Todo | Ongoing | Done
-// preorder: Todo -> Ongoing -> Done
-
-type task_with_status (a: Type) = a & task_status
-
-type mono_list (a: Type) = list (task_with_status a)
-
-(*
-What we need to do:
-- create empty mono_list, with counter 0, empty work_queue
-- add a todo element
-- change a task from 
-*)
 
 //#push-options "--fuel 10 --ifuel 10 --z3rlimit 10"
 let smaller_status: P.preorder task_status =
@@ -36,7 +20,7 @@ match x, y with
 | _, _ -> False
 
 let rec is_same_mono_same_length x y:
-Lemma (is_same_mono_list x y ==> length x = length y)
+Lemma (is_same_mono_list x y ==> L.length x = L.length y)
 = match x, y with
 | _::qx, _::qy -> is_same_mono_same_length qx qy
 | _ -> ()
@@ -53,63 +37,93 @@ Lemma (is_same_mono_list x y /\ is_same_mono_list y z ==> is_same_mono_list x z)
 | _::qx, _::qy, _::qz -> is_same_trans qx qy qz
 | _ -> ()
 
-let rec is_mono_suffix #a (x y: mono_list a): prop
-= if length x < length y then is_mono_suffix x (tl y)
-  else if length x = length y then is_same_mono_list x y
+let rec is_mono_suffix' #a (x y: mono_list a): prop
+= if L.length x < L.length y then is_mono_suffix' x (L.tl y)
+  else if L.length x = L.length y then is_same_mono_list x y
   else False
 
 let is_mono_suffix_refl x:
-Lemma (is_mono_suffix x x)
+Lemma (is_mono_suffix' x x)
 = is_same_refl x
 
 let rec is_mono_suffix_trans x y z:
-Lemma (requires is_mono_suffix x y /\ is_mono_suffix y z)
-(ensures is_mono_suffix x z)
-= if length y < length z then
-    is_mono_suffix_trans x y (tl z)
+Lemma (requires is_mono_suffix' x y /\ is_mono_suffix' y z)
+(ensures is_mono_suffix' x z)
+= if L.length y < L.length z then
+    is_mono_suffix_trans x y (L.tl z)
   else (
-    assert (length y == length z);
-    if length x < length y then
-        is_mono_suffix_trans x (tl y) (tl z)
+    assert (L.length y == L.length z);
+    if L.length x < L.length y then
+        is_mono_suffix_trans x (L.tl y) (L.tl z)
     else is_same_trans x y z
   )
 
-let rec task_in_queue #a (x: a) (l: mono_list a) =
+let is_mono_suffix #a =
+  introduce forall x. (is_mono_suffix' #a x x) with (is_mono_suffix_refl #a x);
+  introduce forall x y z. (is_mono_suffix' #a x y /\ is_mono_suffix' y z
+    ==> is_mono_suffix' x z) with (
+  introduce (is_mono_suffix' #a x y /\ is_mono_suffix' y z)
+    ==> is_mono_suffix' x z
+    with _. (is_mono_suffix_trans x y z)
+  );
+  is_mono_suffix'
+
+// [..., ..., task] -> pos 0
+// [task, ...] -> pos 1
+// l[length l - (pos_task + 1)] = task
+// length l - pos_task - 1 >= 0
+// pos_task < length l
+// if pos_task + 1 == length l --> we're there!
+
+let rec task_in_queue #a (x: a) (pos:nat) (l: mono_list a) =
+  if pos + 1 = L.length l then
+    fst (L.hd l) == x
+  else if pos + 1 < L.length l then
+    task_in_queue x pos (L.tl l)
+  else False
+
+
+  //x == fst (L.index l (L.length l - pos - 1))
+  (*
+  if pos + 1 = length l then // we're there
    match l with
   | [] -> False
   | t::q -> x == fst t \/ task_in_queue x q
+  *)
 
-let rec task_in_queue_same_mono #a (t: a) (x y: mono_list a):
+let rec task_in_queue_same_mono #a (t: a) (pos:nat) (x y: mono_list a):
 Lemma (requires is_same_mono_list x y)
-      (ensures task_in_queue t x ==> task_in_queue t y)
-= match x, y with
-| tx::qx, ty::qy -> task_in_queue_same_mono t qx qy
+      (ensures task_in_queue t pos x ==> task_in_queue t pos y)
+= is_same_mono_same_length x y;
+  if pos + 1 < L.length x then
+    task_in_queue_same_mono t pos (L.tl x) (L.tl y)
+  else ()
+(*
+match x, y with
+| tx::qx, ty::qy -> task_in_queue_same_mono t pos qx qy
 | _ -> ()
+*)
 
 // main reason why we want this preorder:
 let rec task_in_queue_preorder #a 
-    (t: a) (x y: mono_list a):
-Lemma (requires task_in_queue t x /\ is_mono_suffix x y)
-      (ensures task_in_queue t y)
-= if length x < length y then task_in_queue_preorder t x (tl y)
-  else task_in_queue_same_mono t x y
-
-let rec count_ongoing #a (l: mono_list a): nat =
-match l with
-| [] -> 0
-| (_, s)::q -> (if s = Ongoing then 1 else 0) + count_ongoing q
-
-let get_actual_queue #a (l: mono_list a): list a =
-    map fst (filter (fun t -> Todo? (snd t)) l)
+    (t: a) (pos: nat) (x y: mono_list a):
+Lemma (requires task_in_queue t pos x /\ is_mono_suffix x y)
+      (ensures task_in_queue t pos y)
+= if L.length x < L.length y then task_in_queue_preorder t pos x (L.tl y)
+  else task_in_queue_same_mono t pos x y
 
 // 1. enqueue: when spawning a new task
-let enqueue_todo #a (l: mono_list a) (t: a):
+// get a certificate for task_in_queue
+let enqueue_todo #a (l: mono_list a) (t: a)
+(*
 (r:mono_list a{ get_actual_queue r == t::get_actual_queue l
-                /\ count_ongoing r == count_ongoing l })
-= (t, Todo)::l
+                /\ count_ongoing r == count_ongoing l } &
+pos:nat{task_in_queue t pos r})
+*)
+= (| (t, Todo)::l, L.length l |)
 
 let enqueue_preserves_order l t:
-Lemma (is_mono_suffix l (enqueue_todo l t))
+Lemma (is_mono_suffix l (enqueue_todo l t)._1)
 = is_same_refl l
 
 // 2. pop: when a worker starts working on a task
@@ -144,40 +158,147 @@ Lemma (requires ~(get_actual_queue l == []))
 // do I need an id (with distinctness) to compare two tasks?
 // If equality does not work, can add indices, with a uniqueness invariant...
 let rec close_task #a
-    (eq: (x:a -> y:a -> b:bool{b <==> x == y }))
+    //(eq: (x:a -> y:a -> b:bool{b <==> x == y }))
     (t: a)
-    (l: mono_list a{task_in_queue t l}):
-    (s:task_status{memP (t, s) l} & r:mono_list a{
+    (pos: nat)
+    (l: mono_list a{task_in_queue t pos l}):
+    (s:task_status{L.memP (t, s) l} & r:mono_list a{
         s == Ongoing ==> (
             get_actual_queue r == get_actual_queue l /\
             count_ongoing r == count_ongoing l - 1)})
 = match l with
-| (t', s)::q -> if eq t t' then (| s, (t', Done)::q |)
-else let (| s', q' |) = close_task eq t q in (| s', (t', s)::q' |)
+| (t', s)::q -> 
+//if eq t t'
+if pos + 1 = L.length l
+  then (| s, (t', Done)::q |)
+  else let (| s', q' |) = close_task t pos q in (| s', (t', s)::q' |)
 
 let rec close_task_preserves_order_aux #a
-    (eq: (x:a -> y:a -> b:bool{b <==> x == y }))
     (t: a)
-    (l: mono_list a{task_in_queue t l}):
-    Lemma (is_same_mono_list l (close_task eq t l)._2 )
+    (pos: nat)
+    (l: mono_list a{task_in_queue t pos l}):
+    Lemma (is_same_mono_list l (close_task t pos l)._2 )
 = match l with
-| (t', s)::q -> if eq t t' then is_mono_suffix_refl q
-else let (| s', q' |) = close_task eq t q in close_task_preserves_order_aux eq t q
+| (t', s)::q -> if pos + 1 = L.length l then is_mono_suffix_refl q
+else let (| s', q' |) = close_task t pos q in close_task_preserves_order_aux t pos q
 
 let close_task_preserves_order #a
-    (eq: (x:a -> y:a -> b:bool{b <==> x == y }))
     (t: a)
-    (l: mono_list a{task_in_queue t l}):
-    Lemma (is_mono_suffix l (close_task eq t l)._2 )
-= close_task_preserves_order_aux eq t l; from_same_to_suffix l (close_task eq t l)._2
+    (pos: nat)
+    (l: mono_list a{task_in_queue t pos l}):
+    Lemma (is_mono_suffix l (close_task t pos l)._2 )
+= close_task_preserves_order_aux t pos l; from_same_to_suffix l (close_task t pos l)._2
 
+(** Part 2: Instantiation as a ghost monotonic reference **)
+
+module M = Pulse.Lib.GhostMonotonicHigherReference
+open Pulse.Lib.Pervasives
+
+let ghost_mono_ref a = M.ref (mono_list a) is_mono_suffix
+
+let pts_to_ghost_queue #a (r: ghost_mono_ref a) (l: mono_list a): vprop
+= M.pts_to r full_perm l
+
+let alloc_ghost_queue (#a:Type)
+  : stt_ghost (ghost_mono_ref a) emp_inames emp (fun r -> pts_to_ghost_queue r [])
+= M.alloc is_mono_suffix []
+
+let write_ghost_queue (#a:Type) (#v: mono_list a)
+          (r:ghost_mono_ref a) (x: mono_list a)
+  : stt_ghost unit emp_inames (pts_to_ghost_queue r v ** pure (squash (is_mono_suffix v x)))
+               (fun v -> pts_to_ghost_queue r x)
+= M.write r x
+
+let task_in_queue_stable t pos:
+Lemma (P.stable (task_in_queue t pos) is_mono_suffix)
+= introduce forall x y. (task_in_queue t pos x /\ is_mono_suffix x y
+==> task_in_queue t pos y) with
+  (introduce (task_in_queue t pos x /\ is_mono_suffix x y)
+  ==> task_in_queue t pos y with _. task_in_queue_preorder t pos x y)
+
+// can witness that task is in queue
+let witness (#a:Type) #t #pos
+            (r:ghost_mono_ref a)
+            //(fact:stable_property p)
+            (v:erased (mono_list a))
+            (_:squash (task_in_queue t pos v))
+  : //TODO: SteelAtomicUT
+  stt_ghost (M.witnessed r (task_in_queue t pos)) emp_inames
+                  (pts_to_ghost_queue r v)
+                  (fun _ -> pts_to_ghost_queue r v)
+= task_in_queue_stable t pos ; M.witness r (task_in_queue t pos) v _
+
+let recall (#a:Type u#1) #t #pos
+           (r:ghost_mono_ref a)
+           (v:erased (mono_list a))
+           (w:M.witnessed r (task_in_queue t pos))
+  : //TODO: SteelAtomicU
+ stt_ghost unit emp_inames
+                 (pts_to_ghost_queue r v)
+                 (fun _ -> pts_to_ghost_queue r v ** pure (task_in_queue t pos v))
+  = M.recall (task_in_queue t pos) r v w
+
+
+(** Part 3: Associated permissions: Reasoning done here **)
+
+module Lock = Pulse.Lib.SpinLock
+
+unfold
+let one_quart = half_perm (half_perm full_perm)
+
+unfold
+let three_quart = sum_perm (half_perm full_perm) (half_perm (half_perm full_perm))
+
+let own_res (#a: Type0) (r: ref (option a)) = (exists_ (fun v -> pts_to r #one_quart v))
+
+let unit_emp_stt_pure_pure a
+  = unit -> stt a emp (fun _ -> emp)
+
+let task_elem: Type u#1 = (
+  a: Type0 // return type of the computation
+  & r: ref (option a) // the reference where we put the result of the computation
+  & Lock.lock (own_res r)//(exists_ (fun v -> pts_to r half v ** (if None? v then pts_to r half v else emp)))
+  & (unit_emp_stt_pure_pure a)
+)
+
+let task_plus: Type u#1 = task_with_status task_elem
+
+// in NewDomains, g is ._3 and f is ._1
+let task_res_own (t: task_plus): vprop
+= match t._2 with
+| Todo -> pts_to (t._1._2) #three_quart None
+| Ongoing -> emp // in this case, the worker has the half permission
+| Done -> (exists_ (fun v -> pts_to (t._1._2) #three_quart v ** pure (Some? v)))
+
+let mono_list_task_plus: Type u#1 = mono_list task_elem
+  
+let rec tasks_res_own (l: mono_list_task_plus): vprop
+=  match l with
+  | [] -> emp
+  | tl::ql -> task_res_own tl ** tasks_res_own ql
+
+```pulse
+fn fold_done_task (t: task_elem) (l:mono_list_task_plus)
+  requires pts_to t._2 #three_quart None ** tasks_res_own l
+  ensures tasks_res_own (enqueue_todo l t)._1
+{
+  rewrite (pts_to t._2 #three_quart None) as (task_res_own (t, Todo));
+  fold (task_res_own (t, Todo));
+  rewrite (task_res_own (t, Todo) ** tasks_res_own l)
+    as
+  (tasks_res_own (enqueue_todo l t)._1);
+  ()
+}
+```
+
+(*
+Need:
+1. Being able to enqueue, and return witnessed
+2. Being able to pop
+3. Being able to set task to done
+*)
 
 (** We connect the mono list with the actual queue and counter **)
-
-
-
-let pure_inv_queue #a (q: list a) (c: int) (l: mono_list a)
-= count_ongoing l = c /\ get_actual_queue l == q
 
 
 (*
