share/steel/examples/pulse/lib/Pulse.Lib.GhostMonotonicHigherReference.fsti
@@ -1,0 +1,111 @@
+(*
+   Copyright 2020 Microsoft Research
+
+   Licensed under the Apache License, Version 2.0 (the "License");
+   you may not use this file except in compliance with the License.
+   You may obtain a copy of the License at
+
+       http://www.apache.org/licenses/LICENSE-2.0
+
+   Unless required by applicable law or agreed to in writing, software
+   distributed under the License is distributed on an "AS IS" BASIS,
+   WITHOUT WARRANTIES OR CONDITIONS OF ANY KIND, either express or implied.
+   See the License for the specific language governing permissions and
+   limitations under the License.
+*)
+
+module Pulse.Lib.GhostMonotonicHigherReference
+
+open FStar.PCM
+open FStar.Ghost
+//open Steel.FractionalPermission
+
+(*
+open Steel.Memory
+open Steel.Effect.Atomic
+open Steel.Effect
+*)
+open Pulse.Lib.Pervasives
+
+module Preorder = FStar.Preorder
+
+/// A library for Steel references that are monotonic with respect to a user-specified preorder.
+/// This library builds on top of Steel.HigherReference, and is specialized to values at universe 1.
+
+/// An abstract datatype for monotonic references
+[@@erasable]
+val ref (a:Type u#1) (p:Preorder.preorder a)
+  : Type u#0
+
+val pts_to (#a:Type) (#p:Preorder.preorder a) (r:ref a p) (f:perm) (v:a) : vprop
+
+/// Allocates a reference with value [x]. We have full permission on the newly
+/// allocated reference.
+val alloc (#opened: _) (#a:Type) (p:Preorder.preorder a) (v:a)
+  : stt_ghost (ref a p) opened emp (fun r -> pts_to r full_perm v)
+
+/// Writes value [x] in the reference [r], as long as we have full ownership of [r]
+val write (#opened: _) (#a:Type) (#p:Preorder.preorder a) (#v:a)
+          (r:ref a p) (x:a)
+  : stt_ghost unit opened (pts_to r full_perm v ** pure (squash (p v x)))
+               (fun v -> pts_to r full_perm x)
+
+/// A wrapper around a predicate that depends on a value of type [a]
+let property (a:Type)
+  = a -> prop
+
+/// A wrapper around a property [fact] that has been witnessed to be true and stable
+/// with respect to preorder [p]
+val witnessed (#a:Type u#1) (#p:Preorder.preorder a) (r:ref a p) (fact:property a)
+  : Type0
+
+/// The type of properties depending on values of type [a], and that
+/// are stable with respect to the preorder [p]
+let stable_property (#a:Type) (p:Preorder.preorder a)
+  = fact:property a { Preorder.stable fact p }
+
+/// If [fact] is a stable property for the reference preorder [p], and if
+/// it holds for the current value [v] of the reference, then we can witness it
+val witness (#inames: _) (#a:Type) (#q:perm) (#p:Preorder.preorder a) (r:ref a p)
+            (fact:stable_property p)
+            (v:erased a)
+            (_:squash (fact v))
+  : //TODO: SteelAtomicUT
+  stt_ghost (witnessed r fact) inames
+                  (pts_to r q v)
+                  (fun _ -> pts_to r q v)
+
+
+/// If we previously witnessed the validity of [fact], we can recall its validity
+val recall (#inames: _) (#a:Type u#1) (#q:perm) (#p:Preorder.preorder a)
+           (fact:property a)
+           (r:ref a p)
+           (v:erased a)
+           (w:witnessed r fact)
+  : //TODO: SteelAtomicU
+ stt_ghost unit inames
+                 (pts_to r q v)
+                 (fun _ -> pts_to r q v ** pure (fact v))
+
+/// Monotonic references are also equipped with the usual fractional permission discipline
+/// So, you can split a reference into two read-only shares
+val share (#inames:_)
+          (#a:Type)
+          (#p:Preorder.preorder a)
+          (r:ref a p)
+          (f:perm)
+          (v:a)
+  : stt_ghost unit inames
+    (pts_to r f v)
+    (fun _ -> pts_to r (half_perm f) v ** pts_to r (half_perm f) v)
+
+/// And you can gather back the shares
+val gather (#inames:_)
+           (#a:Type)
+           (#p:Preorder.preorder a)
+           (r:ref a p)
+           (f g:perm)
+           (v:a)
+  : stt_ghost unit inames
+    (pts_to r f v ** pts_to r g v)
+    (fun _ -> pts_to r (sum_perm f g) v)
