share/steel/examples/pulse/parallel/GhostTaskQueue.fsti
@@ -1,0 +1,73 @@
+module GhostTaskQueue
+
+module L = FStar.List.Tot.Base
+module P = FStar.Preorder
+
+// Mostly: Monotonic list of tasks with status
+type task_status = | Todo | Ongoing | Done
+// preorder: Todo -> Ongoing -> Done
+
+type task_with_status (a: Type) = a & task_status
+type mono_list (a: Type) = list (task_with_status a)
+
+// the list can only evolve according to this order
+// it imposes todo < ongoing < done, which we do not use
+val is_mono_suffix (#a: Type): P.preorder (mono_list a)
+
+val task_in_queue (#a: Type) (x: a) (pos:nat) (l: mono_list a): prop
+
+val task_in_queue_preorder (#a: Type)
+    (t: a) (pos: nat) (x y: mono_list a):
+Lemma (requires task_in_queue t pos x /\ is_mono_suffix x y)
+      (ensures task_in_queue t pos y)
+
+let rec count_ongoing #a (l: mono_list a): nat =
+match l with
+| [] -> 0
+| (_, s)::q -> (if s = Ongoing then 1 else 0) + count_ongoing q
+
+let get_actual_queue #a (l: mono_list a): list a =
+    L.map fst (L.filter (fun t -> Todo? (snd t)) l)
+
+// 1. enqueue: when spawning a new task
+// get a certificate for task_in_queue
+val enqueue_todo (#a: Type) (l: mono_list a) (t: a):
+(r:mono_list a{ get_actual_queue r == t::get_actual_queue l
+                /\ count_ongoing r == count_ongoing l
+                /\ r == (t, Todo)::l } &
+pos:nat{task_in_queue t pos r})
+
+val enqueue_preserves_order (#a: Type) (l: mono_list a) (t: a):
+Lemma (is_mono_suffix l (enqueue_todo l t)._1)
+
+// 2. pop: when a worker starts working on a task
+// it updates the task to "ongoing"
+val pop_todo_task (#a: Type) (l: mono_list a{~(get_actual_queue l == [])})
+: (t:a & r:mono_list a{ get_actual_queue l == t::get_actual_queue r
+                /\ count_ongoing r == count_ongoing l + 1 })
+
+val pop_preserves_order (#a: Type) (l: mono_list a):
+Lemma (requires ~(get_actual_queue l == []))
+      (ensures is_mono_suffix l (pop_todo_task l)._2)
+
+(** 3. concluding the task: when the worker is done **)
+// a bit weird: Can we prove the task was not done before???
+// yes, because we have the permission?
+// maybe with 2/3 + 2/3 permissions
+val close_task (#a: Type)
+    (t: a)
+    (pos: nat)
+    (l: mono_list a{task_in_queue t pos l})
+  : (s:task_status{L.memP (t, s) l} & r:mono_list a{
+        s == Ongoing ==> (
+            get_actual_queue r == get_actual_queue l /\
+            count_ongoing r == count_ongoing l - 1)})
+
+val close_task_preserves_order (#a: Type)
+    (t: a) (pos: nat) (l: mono_list a{task_in_queue t pos l}):
+    Lemma (is_mono_suffix l (close_task t pos l)._2 )
+
+(** We connect the mono list with the actual queue and counter **)
+
+let pure_inv_queue #a (q: list a) (c: int) (l: mono_list a)
+= count_ongoing l = c /\ get_actual_queue l == q
